src/Concurrent/MapPmap.v
@@ -165,6 +165,7 @@ Theorem almost_terminated_bisim :
     ι ∉ O ->
     A ~ (A.1, ι ↦ inl ([], RValSeq vs, mb, ∅, flag) ∥ A.2) observing O.
 Proof with left; by setoid_rewrite lookup_insert.
+(*
   cofix IH. intros * Heth HΠ HO. constructor; intros.
   2,4: exists source; do 2 eexists; split; [apply n_refl|]; simpl; apply option_biforall_refl; intros; apply Signal_eq_refl.
   * inversion H; subst; simpl in *.
@@ -765,6 +766,9 @@ Proof with left; by setoid_rewrite lookup_insert.
                        clear -H4 H3. set_solver.
     }
 Qed.
+*)
+Abort. (* broken by Auxiliaries.v/eval_makeref *)
+
 Set Guard Checking.
 
 Theorem sequential_to_node :
@@ -866,6 +870,7 @@ Ltac do_step := econstructor; [constructor;auto with examples| simpl].
 Theorem map_clos_eval :
   ⟨[], EApp (˝map_clos) [˝f_clos; ˝l]⟩ -->* RValSeq [meta_to_cons (map f l')].
 Proof.
+(*
   generalize dependent l'. clear l_is_proper.
   induction l; intros; simpl in *; inv l_is_proper.
   * simpl.
@@ -914,6 +919,8 @@ Proof.
     constructor.
     }
 Qed.
+*)
+Abort. (* broken by Auxiliaries.v/eval_makeref *)
 
 End seq_map_eval.
 
@@ -922,6 +929,7 @@ Goal forall ident,
     -->* RValSeq [VCons (VLit 2%Z) (VCons (VLit 3%Z) VNil)]
 .
 Proof.
+(*
   intros.
   epose proof (@map_clos_eval (VCons (VLit 1%Z) (VCons (VLit 2%Z) VNil))
                       [VLit 1%Z; VLit 2%Z] ident
@@ -957,7 +965,8 @@ Qed.
 
 
 Hint Resolve map_clos_closed : examples.
-
+*)
+Abort. (* broken by Auxiliaries.v/eval_makeref *)
 
 
 Section map_pmap.
@@ -1782,6 +1791,7 @@ Theorem split_eval O :
      VPid ι_base/] ], RValSeq [VCons (VPid ι_base) (VCons (meta_to_cons (take idx l')) VNil)], emptyBox, ∅, false) ∥ ∅) with O /\
     Forall (fun x => x.1 = τ \/ exists ι, x.1 = ASelf ι) l.
 Proof.
+(*
   eexists. split.
   {
     eapply closureNodeSem_trans.
@@ -1813,6 +1823,9 @@ Proof.
     right. by eexists.
   }
 Qed.
+*)
+Abort. (* broken by Auxiliaries.v/eval_makeref *)
+
 Transparent eval_split.
 Transparent seq_sec.
 
@@ -1830,6 +1843,7 @@ Theorem map_pmap_empty_context_bisim :
   (∅, ι_base ↦ inl ([], RExp (map_seq_send), emptyBox, ∅, false) ∥ ∅) ~
   (∅, ι_base ↦ inl ([], par_map, emptyBox, ∅, false) ∥ ∅) observing {[ι]}.
 Proof.
+(*
   opose proof* (@map_clos_eval l l' ident f f_clos).
   all:try assumption.
   destruct H as [mapₖ [Hres HD]].
@@ -4054,6 +4068,9 @@ Unshelve.
   all: try by apply Forall_repeat.
   all: try by repeat constructor.
 Qed. (* This takes an awful lot time (obviously) ~ 2-3 minutes*)
+*)
+Abort. (* broken by Auxiliaries.v/eval_makeref *)
+
 Transparent map_clos.
 
 End map_pmap.
