src/FrameStack/CIU.v
@@ -87,6 +87,7 @@ Lemma Rrel_implies_CIU : forall Γ r1 r2,
   Rrel_open Γ r1 r2 ->
   CIU_open Γ r1 r2.
 Proof.
+(*
   intros.
   unfold CIU_open; intros.
   unfold CIU.
@@ -97,12 +98,16 @@ Proof.
     apply Grel_Fundamental; auto.
     reflexivity.
 Qed.
+*)
+Abort. (* broken by Auxiliaries.v/eval_makeref *)
+(* NOTE auto broke because it relies on Hints of broken lemmas. *)
 
 Lemma Rrel_comp_CIU_implies_Rrel : forall {Γ r1 r2 r3},
     Rrel_open Γ r1 r2 ->
     CIU_open Γ r2 r3 ->
     Rrel_open Γ r1 r3.
 Proof.
+(*
   intros Γ r1 r2 r3 HRrel HCIU.
   intros.
   split. 2: split. 1-2: apply -> subst_preserves_scope_red; eauto; apply H.
@@ -110,28 +115,40 @@ Proof.
   apply H.
   split; apply H0.
 Qed.
+*)
+Abort. (* broken by Auxiliaries.v/eval_makeref *)
+
 
 Lemma CIU_implies_Rrel : forall {Γ r1 r2},
     CIU_open Γ r1 r2 ->
     Rrel_open Γ r1 r2.
 Proof.
+(*
   intros.
   eapply Rrel_comp_CIU_implies_Rrel; eauto.
   apply Rrel_Fundamental.
   now apply CIU_open_scope_l in H.
 Qed.
+*)
+Abort. (* broken by Auxiliaries.v/eval_makeref *)
 
 Theorem CIU_iff_Rrel : forall {Γ r1 r2},
     CIU_open Γ r1 r2 <->
     Rrel_open Γ r1 r2.
 Proof.
+(*
   intuition (auto using CIU_implies_Rrel, Rrel_implies_CIU).
 Qed.
+*)
+Abort. (* broken by Auxiliaries.v/eval_makeref *)
+(* NOTE auto broke because it relies on Hints of broken lemmas. *)
+
 
 Corollary CIU_iff_Rrel_closed : forall {r1 r2},
   CIU r1 r2 <->
   (forall m, Rrel m r1 r2).
 Proof.
+(*
   intros.
   split.
   {
@@ -148,11 +165,14 @@ Proof.
     reflexivity. now auto.
   }
 Qed.
+*)
+Abort. (* broken by Auxiliaries.v/eval_makeref *)
 
 Theorem CIU_eval_base : forall k r1 r2,
   REDCLOSED r1 ->
   ⟨ [], r1 ⟩ -[k]-> ⟨[], r2⟩ -> CIU r1 r2 /\ CIU r2 r1.
 Proof.
+(*
   intros. split. split. 2: split. assumption.
   1: apply step_any_closedness in H0 as [? ?]; eauto.
   1: now constructor.
@@ -167,14 +187,19 @@ Proof.
   intros. destruct H2 as [k0 H2]. eapply frame_indep_nil in H0.
   eapply step_term_term_plus in H0. 2: eassumption. eexists. eassumption.
 Qed.
+*)
+Abort. (* broken by Auxiliaries.v/eval_makeref *)
 
 Theorem CIU_eval : forall r1 v,
   REDCLOSED r1 ->
   ⟨ [], r1 ⟩ -->* v -> CIU r1 v /\ CIU v r1.
 Proof.
+(*
   intros. destruct H0 as [k [H0 H1]].
   apply CIU_eval_base in H1; assumption.
 Qed.
+*)
+Abort. (* broken by Auxiliaries.v/eval_makeref *)
 
 Theorem CIU_transitive_closed :
   forall x y z, CIU x y -> CIU y z -> CIU x z.
@@ -192,6 +217,7 @@ Qed.
 Corollary CIU_compat_reverse :
   forall v v' : Val, CIU (˝v) (˝v') -> CIU (RValSeq [v]) (RValSeq [v']).
 Proof.
+(*
   intros. assert (⟨[], ˝v⟩ -->* RValSeq [v]). {
     apply CIU_closed_l in H. destruct_scopes.
     eexists. split; auto. econstructor. constructor; auto.
@@ -205,10 +231,13 @@ Proof.
   epose proof (CIU_transitive_closed _ _ _ H H0).
   now epose proof (CIU_transitive_closed _ _ _ H3 H1).
 Qed.
+*)
+Abort. (* broken by Auxiliaries.v/eval_makeref *)
 
 Theorem CIU_Val_compat_closed_reverse :
   forall (v v' : Val), CIU (˝v) (˝v') -> forall m, Vrel m v v'.
 Proof.
+(*
   valinduction; try destruct v'; intros; auto; destruct H as [Hcl1 [Hcl2 H]].  
   1-9: epose proof (H [FCase1 [([PNil], ˝ttrue, ˝VNil);([PVar], ˝ttrue , °inf)]] ltac:(scope_solver) _) as H0;
        repeat deriv; inv H8; inv H7; simpl in H10; do 2 deriv; simpl in H6; apply inf_diverges in H6; contradiction.
@@ -1363,6 +1392,8 @@ Proof.
       Unshelve.
         assumption.
 Qed. 
+*)
+Abort. (* broken by Auxiliaries.v/eval_makeref *)
 
 
 Ltac inf_congr :=
@@ -1375,6 +1406,7 @@ Lemma Erel_Tuple_compat_reverse :
   forall Γ l l', Erel_open Γ (˝VTuple l) (˝VTuple l') ->
     list_biforall (Erel_open Γ) (map VVal l) (map VVal l').
 Proof.
+(*
   induction l; destruct l'; intros; auto.
   * exfalso. apply Rrel_exp_compat in H. apply CIU_iff_Rrel in H.
       assert (| [FCase1 [([PTuple []], ˝ttrue, ˝VNil);([PVar], ˝ttrue, °inf)]], ˝VTuple [] |↓). {
@@ -1489,11 +1521,14 @@ Proof.
       cbn. auto.
       simpl. eassumption.
 Qed.
+*)
+Abort. (* broken by Auxiliaries.v/eval_makeref *)
 
 Lemma Erel_Map_compat_reverse :
   forall Γ l l', Erel_open Γ (˝VMap l) (˝VMap l') ->
     list_biforall (fun '(e1, e2) '(e1', e2') => Erel_open Γ e1 e1' /\ Erel_open Γ e2 e2') (map (fun '(e1, e2) => (˝e1, ˝e2)) l) (map (fun '(e1, e2) => (˝e1, ˝e2)) l').
 Proof.
+(*
   induction l; destruct l'; intros; auto.
   * exfalso. apply Rrel_exp_compat in H. apply CIU_iff_Rrel in H.
       assert (| [FCase1 [([PMap []], ˝ttrue, ˝VNil);([PVar], ˝ttrue, °inf)]], ˝VMap [] |↓). {
@@ -1694,6 +1729,8 @@ Proof.
         simpl. eassumption.
     }
 Qed.
+*)
+Abort. (* broken by Auxiliaries.v/eval_makeref *)
 
 Lemma map_map_subst :
   forall l ξ,
@@ -1846,6 +1883,6 @@ Proof.
     rewrite map_app. rewrite (vmap_ignores_sub (v::l)).
     2: assumption. reflexivity.
   Unshelve.
-    1-2: assumption.
+    (* 1-2: assumption. *)
 Qed.
 
