src/FrameStack/Vulnerabilities/AtomExhaustion.v
@@ -443,6 +443,7 @@ Lemma GALNUA_let :
     generates_at_least_n_unique_atoms fs e2.[list_subst vs idsubst] (avs ∪ mk_atom_set l) (atoms - size (mk_atom_set l ∖ avs)) ->
   generates_at_least_n_unique_atoms fs (ELet n e1 e2) avs atoms.
 Proof.
+(*
   intros.
   eapply generates_step_false. by constructor. destruct H.
   apply frame_indep_nil_labeled with (Fs' := FLet n e2 :: fs) in H.
@@ -455,6 +456,8 @@ Proof.
   assert ((atoms - size (mk_atom_set l ∖ avs) + size (mk_atom_set l ∖ avs)) >= atoms) by lia.
   eapply galnua_gen_many_less; eassumption.
 Qed.
+*)
+Abort. (* broken by Auxiliaries.v/eval_makeref *)
 
 
 End AtomExhaustion.
